src/tls/ParsersAux.ClientHelloExtension.fsti
@@ -1,0 +1,14 @@
+module ParsersAux.ClientHelloExtension
+include Parsers.ClientHelloExtension
+
+module Seq = FStar.Seq
+module LP = LowParse.Low.Base
+module CHE = Parsers.ClientHelloExtension
+module ET = Parsers.ExtensionType
+
+val serialize_clientHelloExtension_eq_pre_shared_key
+  (e: CHE.clientHelloExtension {CHE.CHE_pre_shared_key? e})
+: Lemma
+  (LP.serialize CHE.clientHelloExtension_serializer e ==
+   LP.serialize ET.extensionType_serializer ET.Pre_shared_key `Seq.append`
+   LP.serialize CHE.clientHelloExtension_CHE_pre_shared_key_serializer (CHE.CHE_pre_shared_key?._0 e))
